working on switch compilation, quite slow going

src/Fmajortoemajor.v
@@ -60,6 +60,139 @@ let transf_cases (targid : ident) (cases : list (Z * Fmajor.stmt)) (target_d : E
   | Fmajor.Sswitch targid cases target => transf_cases targid cases (transf_expr target)
   end.
 
+Definition transf_cases (targid : ident) (cases : list (Z * Fmajor.stmt)) (target_d : Emajor.expr) :=
+  let fix mk_cases (i : nat) (cases : list (Z * Fmajor.stmt)) : list (Z * nat) :=
+      match cases with
+      | [] => []
+      | (v, s) :: cases => (v, i) :: mk_cases (S i) cases
+      end in
+    let switch := Emajor.Sswitch targid target_d (mk_cases 0%nat cases) (length cases) in
+    let swblock := Emajor.Sblock switch in
+    let fix mk_blocks (acc : Emajor.stmt) (i : nat) (cases : list (Z * Fmajor.stmt)) :=
+        match cases with
+        | [] => acc
+        | (v, s) :: cases =>
+                let acc' :=
+                    Emajor.Sblock (Emajor.Sseq acc
+                                  (Emajor.Sseq (transf_stmt s)
+                                               (Emajor.Sexit (length cases - i)))) in
+                mk_blocks acc' (S i) cases
+        end in
+    mk_blocks swblock 0%nat cases.
+
+Fixpoint mk_cases (i : nat) (cases : list (Z * Fmajor.stmt)) : list (Z * nat) :=
+  match cases with
+  | [] => []
+  | (v, s) :: cases => (v, i) :: mk_cases (S i) cases
+  end.
+
+Fixpoint mk_blocks (acc : Emajor.stmt) (i : nat) (cases : list (Z * Fmajor.stmt)) :=
+  match cases with
+  | [] => acc
+  | (v, s) :: cases =>
+    let acc' :=
+        Emajor.Sblock (Emajor.Sseq acc
+                                   (Emajor.Sseq (transf_stmt s)
+                                                (Emajor.Sexit (length cases - i)))) in
+    mk_blocks acc' (S i) cases
+  end.
+
+(* Here is the base problem *)
+(* We need to rewrite all the transformations to not be tail recursive *)
+(* Just mk_blocks then *)
+
+Fixpoint mk_blocks_no_acc (base : Emajor.stmt) (i : nat) (cases : list (Z * Fmajor.stmt)) :=
+  match cases with
+  | [] => base
+  | (v,s) :: cases =>
+    let r := mk_blocks_no_acc base (S i) cases in
+    Emajor.Sblock (Emajor.Sseq r
+                                 (Emajor.Sseq (transf_stmt s)
+                                              (Emajor.Sexit (i - length cases))))
+  end.
+
+(*
+Definition base := Emajor.SmakeConstr xH Int.zero nil.
+Definition cases := [(12,Fmajor.Sassign xH (Fmajor.Var xH));(24,Fmajor.Sseq Fmajor.Sskip Fmajor.Sskip);(18, Fmajor.Sskip);(3, Fmajor.Sskip);(6, Fmajor.Sskip)].
+
+Definition mb := mk_blocks base O cases.
+Definition mbna := mk_blocks_no_acc base O (rev cases).
+
+Lemma x :
+  mb = mbna.
+Proof.
+  unfold mb, mbna.
+  simpl.
+  repeat f_equal.
+Qed.
+ *)
+
+Lemma mk_blocks_rev_ind_case_succ :
+  forall l b n z s,
+    mk_blocks b (S n) (l ++ [(z,s)]) = Sblock (Sseq (mk_blocks b n l) (Sseq (transf_stmt s) (Sexit 0))).
+Proof.
+  induction l; intros; simpl;
+    try reflexivity. 
+  destruct a. simpl. rewrite IHl. rewrite app_length. simpl.
+  replace (length l + 1 - S n)%nat with (length l - n)%nat  by omega.
+  reflexivity.
+Qed.
+
+Lemma mk_blocks_no_acc_spec :
+  forall cases b n,
+    mk_blocks b n (rev cases) = mk_blocks_no_acc b n cases.
+Proof.
+  induction cases; intros.
+  simpl. reflexivity.
+  simpl. destruct a.
+  rewrite <- IHcases.
+Admitted.
+  
+
+(*
+Lemma mk_blocks_rev_ind_case_zero :
+  forall l b n z s,
+    mk_blocks b O (l ++ [(z,s)]) = Sblock (Sseq (mk_blocks b n l) (Sseq (transf_stmt s) (Sexit 0))).
+Proof.
+  induction l; intros; simpl;
+    try reflexivity. 
+  destruct a. simpl.
+  rewrite IHl. rewrite app_length. simpl.
+  replace (length l + 1 - S n)%nat with (length l - n)%nat  by omega.
+  reflexivity.
+
+  
+
+Lemma mk_blocks_acc_rev :
+  forall cases base n,
+    mk_blocks base n (rev cases) = mk_blocks_no_acc base n cases.
+Proof.
+  induction cases; intros; try solve [unfold mk_blocks, mk_blocks_no_acc; simpl; reflexivity].
+  simpl.
+  
+  destruct a.
+  destruct n; simpl. rewrite <- IHcases.
+  
+  rewrite mk_blocks_rev_ind_case.
+  
+  rewrite IHcases.
+  simpl.
+
+
+Lemma mk_blocks_acc_rev :
+  forall cases s n,
+    mk_blocks s n cases = mk_blocks_no_acc s (length cases - n) (rev cases).
+Proof.
+  induction cases; intros.
+  simpl; reflexivity.
+  simpl. destruct a.
+  intros. replace (mk_blocks s n cases) with (mk_blocks s n (rev (rev cases))) by (rewrite rev_involutive; eauto).
+  generalize dependent n.
+  generalize dependent s.
+*)  
+
+
+  
 Definition transf_fun_body (f : (Fmajor.stmt * Fmajor.expr)) : Emajor.stmt :=
   let (s,e) := f in
   Sseq (transf_stmt s) (Sreturn (transf_expr e)).
@@ -71,6 +204,24 @@ Definition transf_fundef (f : Fmajor.function) : Emajor.fundef :=
 Definition transf_program (p : Fmajor.program) : Emajor.program :=
   AST.transform_program transf_fundef p.
 
+Lemma transf_switch :
+  forall targid cases target,
+    transf_stmt (Fmajor.Sswitch targid cases target) =
+    transf_cases targid cases (transf_expr target).
+Proof.
+  reflexivity.
+Qed.
+
+Lemma transf_cases_ind_defns :
+  forall targid cases target swblock ncases,
+    ncases = mk_cases O cases ->
+    swblock = Emajor.Sblock (Emajor.Sswitch targid target ncases (length cases)) ->
+    transf_cases targid cases target = mk_blocks swblock O cases.
+Proof.
+  intros. unfold transf_cases. fold mk_blocks. fold mk_cases. subst. reflexivity.
+Qed.
+
+
 Section PRESERVATION.
 
 Variable prog: Fmajor.program.
@@ -79,13 +230,17 @@ Let ge := Genv.globalenv prog.
 Let tge := Genv.globalenv tprog.
 Hypothesis TRANSF : transf_program prog = tprog.
 
-(* We need to wrap up which thing is getting returned in the match_cont? *)
-(* We need to wrap that up somewhere *)
-
+(* The Emajor continuation will have a lot more going on *)
+(* It could have arbitrarily many Kblocks stuck in whenever *)
+(* Somewhere we need to record more precise info *)
 
 Inductive match_cont: Fmajor.cont -> Emajor.cont -> Prop :=
 | match_stop :
     match_cont Fmajor.Kstop Emajor.Kstop
+(* | match_block : (* IS this the right way ? *) *)
+(*     forall k k' s, *)
+(*       match_cont k k' -> *)
+(*       match_cont k (Emajor.Kblock (Emajor.Kseq s k')) *)
 | match_return :
     forall k k' exp,
       match_cont k k' ->
@@ -100,7 +255,14 @@ Inductive match_cont: Fmajor.cont -> Emajor.cont -> Prop :=
       match_cont k k' ->
       match_cont (Fmajor.Kcall id exp f env k) (Emajor.Kcall id (transf_fundef f) env k').
 
-  
+
+Inductive wf_cont : list Fmajor.stmt -> Fmajor.cont -> Emajor.cont -> Prop :=
+| wf_zero : forall k k',
+    match_cont k k' -> wf_cont nil k k'
+| wf_succ : forall k k' l s,
+    wf_cont l k k' ->
+    wf_cont (s :: l) k (Emajor.Kblock (Emajor.Kseq (transf_stmt s) k')).
+
 Inductive match_states: Fmajor.state -> Emajor.state -> Prop :=
 | match_state :
     forall f f' s s' k k' e env,
@@ -112,6 +274,63 @@ Inductive match_states: Fmajor.state -> Emajor.state -> Prop :=
     forall v k k',
       match_cont k k' ->
       match_states (Fmajor.Returnstate v k) (Emajor.Returnstate v k').
+
+(*
+Lemma step_wf_cont :
+  forall targid cases target f sw e k env k' env' sF sE sF',
+    sw = (Fmajor.Sswitch targid cases target) ->
+    sF = (Fmajor.State f sw e k env) ->
+    sE = (Emajor.State (transf_fundef f) (transf_stmt sw) k' env') ->
+    match_states sF sE ->
+    Fmajor.step ge sF E0 sF' ->
+    exists sE',
+      plus Emajor.step tge sE E0 sE' /\ wf_cont (map snd cases) k k'.
+Proof.
+  induction cases; intros; subst.
+  inv H3. simpl in H10. congruence.
+  inversion H2. subst. clear H11.
+  rewrite transf_switch.
+  remember (mk_cases O cases) as ncases.
+  remember (Emajor.Sblock (Emajor.Sswitch targid (transf_expr target) ncases (length cases))) as swblock.
+  erewrite transf_cases_ind_defns; eauto.
+  simpl. destruct a.
+  eexists; split.
+  eapply plus_left; nil_trace.
+  
+  
+Qed.
+  
+
+(* *)
+Lemma step_transf_switch :
+  forall cases targid target f k env tag vargs s,
+    find_case (Int.unsigned tag) cases = Some s ->
+    Fmajor.eval_expr env target (Constr tag vargs) ->
+    exists k' env',
+      plus Emajor.step tge (State f (transf_stmt (Fmajor.Sswitch targid cases target)) k env) E0
+           (State f (transf_stmt s) k' env').
+Proof.
+  induction cases; intros.
+  simpl in H. inv H.
+  simpl in H. repeat (break_match_hyp; try congruence).
+  + subst.
+    inv H.
+    (* Here the statement we wanted is first *)
+    (* This is not near strong enough *)
+Qed.
+*)
+Lemma step_switch :
+  forall targid cases target f sw e k env k' env' sF sE sF',
+    sw = (Fmajor.Sswitch targid cases target) ->
+    sF = (Fmajor.State f sw e k env) ->
+    sE = (Emajor.State (transf_fundef f) (transf_stmt sw) k' env') ->
+    match_states sF sE ->
+    Fmajor.step ge sF E0 sF' ->
+    exists sE',
+      plus Emajor.step tge sE E0 sE' /\ match_states sF' sE'.
+Proof.
+  
+Admitted.
 
 Lemma eval_expr_transf :
   forall env exp v,
@@ -156,6 +375,7 @@ Proof.
   erewrite Genv.find_funct_ptr_transf; eauto.
 Qed.
 
+  
 Lemma step_sim_nil_trace :
   forall (s1 s1' : Fmajor.state) (s2 : Emajor.state),
     match_states s1 s2 ->
@@ -254,7 +474,7 @@ Proof.
     econstructor; eauto.
 
   (* switch *)
-  + admit.
+  + eapply step_switch in H; eauto.
 
   (* Returnstate *)
   + inv H5.
@@ -265,7 +485,7 @@ Proof.
     econstructor; eauto.
     econstructor; eauto.
     
-Admitted.
+Qed.
 
 Lemma step_sim :
   forall (s1 s1' : Fmajor.state) (s2 : Emajor.state) t,
@@ -280,9 +500,34 @@ Proof.
   eapply step_sim_nil_trace; eauto.
 Qed.
 
+Lemma initial_states_match :
+  forall s1,
+    Fmajor.initial_state prog s1 ->
+    exists s2, Emajor.initial_state tprog s2 /\ match_states s1 s2.
+Proof.
+Admitted.
+
+Lemma match_final_states :
+  forall s1 s2 r,
+    match_states s1 s2 ->
+    Fmajor.final_state s1 r ->
+    Emajor.final_state s2 r.
+Proof.
+Admitted.
+
 Theorem fsim :
   forward_simulation (Fmajor.semantics prog) (Emajor.semantics tprog).
 Proof.
-Admitted.
+  eapply forward_simulation_plus.
+  intros. simpl.
+  unfold transf_program in *. subst tprog.
+  solve [eapply Genv.public_symbol_transf].
+
+  solve [eapply initial_states_match; eauto].
+  solve [eapply match_final_states; eauto].
+
+  intros. eapply step_sim; eauto.
+  
+Qed.
   
 End PRESERVATION.
